Test/Interpreter/Felt/unnamed.mlir
@@ -1,6 +1,7 @@
 // RUN: not veir-interpret %s 2>&1 | filecheck %s
 
-// CHECK: Error while interpreting module
+// CHECK:      error: failed to interpret operation
+// CHECK-NEXT:     %c = "felt.const"() <{value = #felt<const 42> : !felt.type}> : () -> !felt.type
 "builtin.module"() ({
   "func.func"() <{sym_name = "main", function_type = () -> !felt.type}> ({
     %c = "felt.const"() <{value = #felt<const 42> : !felt.type}> : () -> !felt.type
